LTS.thy
@@ -4,139 +4,136 @@ imports Main
 
 begin
 
-section {* Execution models *}
+section {* Labeled transition systems and their executions *}
 
 subsection {* Labeled transition systems *}
 
-text {* The semantics of a B component is a discrete, eventful, state-transition systems. We 
-first define what is meant exactly by such systems. Any system is, at a given time in a state. 
-Conversely, a system has a set of possible states. A system evolves from state to state,
-and such changes called transitions. The following record definition of 
-@{text "('st, 'ev) Tr}"} models transitions, where the parametric sorts @{text "'st"} 
-and @{text "'ev"} represent states and events, respectively. *}
+text {* 
+  The semantics of a B component is a discrete, eventful, state-transition systems. We 
+  start by defining labeled transition systems and their behaviors, independently of B.
+  An LTS is given by a set of initial states and a set of transitions, which are
+  triples (source and destination state, and a transition label). The following
+  definitions of transitions and transition systems are parameterized by types
+  @{text "'st"} and @{text "'ev"} of states and events.
+*}
 
 record ('st, 'ev) Tr =
-  src :: 'st -- "source state"
-  dst :: 'st -- "destination state"
-  lbl :: 'ev -- "labeling event"
-
-text {* Building on this formalization of transitions, the record @{text "('st, 'ev) LTS"} 
-formalizes labeled transition systems (LTS):  *}
+  src :: 'st     -- "source state"
+  dst :: 'st     -- "destination state"
+  lbl :: 'ev     -- "labeling event"
 
 record ('st, 'ev) LTS =
   init :: "'st set" -- "set of initial states"
   trans :: "('st, 'ev) Tr set" -- "set of transitions"
 
-text {* The inductively defined set @{term "states"} yields the reachable states of a 
-given LTS. *}
+text {* 
+  The inductively defined set @{term "states m"} corresponds to the set of
+  reachable states of a given LTS @{text m}. 
+*}
 
-inductive_set states :: "('st, 'ev) LTS \<Rightarrow> 'st set" for m :: "('st, 'ev) LTS" where
-  base[elim!]: "s \<in> init m \<Longrightarrow> s \<in> states m"
-| step[elim!]: "\<lbrakk> t \<in> trans m; src t \<in> states m \<rbrakk> \<Longrightarrow> dst t \<in> states m"
-  
-text {* A few lemmas related to reachable states are then enunciated and proved. 
-First, all the initial states are reachable states:*}
+inductive_set states :: "('st, 'ev) LTS \<Rightarrow> 'st set" 
+  for l :: "('st, 'ev) LTS" where
+  base[elim!]: "s \<in> init l \<Longrightarrow> s \<in> states l"
+| step[elim!]: "\<lbrakk> t \<in> trans l; src t \<in> states l \<rbrakk> \<Longrightarrow> dst t \<in> states l"
 
-lemma reachable_init: "init m \<subseteq> states m" 
+inductive_cases base : "s \<in> states l"
+inductive_cases step : "dst t \<in> states l"
+
+text {* 
+  A few lemmas related to reachable states are then enunciated and proved. 
+  First, all the initial states are reachable states:
+*}
+
+lemma reachable_init: "init l \<subseteq> states l"
   by auto
 
 text {* Next, the successors states of the reachable states are themselves reachable states.
 We first define a function @{text "successors"} that returns the set of successors of a
-given set @{text "S"} of states in a given LTS @{text "L"}: *}
+given set @{text "S"} of states in a given LTS @{text "l"}: *}
 
 definition successors :: "('st, 'ev) LTS \<Rightarrow> 'st set \<Rightarrow> 'st set" where
-  "successors m S \<equiv> { dst t | t . t \<in> trans m \<and> src t \<in> S }"
+  "successors l S \<equiv> { dst t | t . t \<in> trans l \<and> src t \<in> S }"
 
 text {* Next, we show that the successors of the reachable states are also reachable. *}
 
-lemma reachable_stable: "successors m (states m) \<subseteq> states m"
+lemma reachable_stable: "successors l (states l) \<subseteq> states l"
   unfolding successors_def by auto
   
-text {* The following lemma is related to the identification of sufficient conditions to establish 
-safety properties. Consider a property that is satisfied by some set of states $S$. If the initial 
-states are in $S$, and if the successors of $S$ are in $S$ then all the reachable states are in 
-$S$. *}
+text {* 
+  The following lemma is at the basis of proofs of invariants, and more
+  generally, safety properties. Any set @{text S} that contains all initial
+  states and is closed under successors contains all reachable states.
+*}
 
 lemma reachable_induct_set:
-  assumes s: "s \<in> states m" and base: "init m \<subseteq> S" and step: "successors m S \<subseteq> S"
+  assumes base: "init l \<subseteq> S"
+  and step: "successors l S \<subseteq> S"
+  and s: "s \<in> states l"
   shows "s \<in> S"
-using s proof (induct s)
-  fix i
-  assume "i \<in> init m"
-  with base show "i \<in> S" ..
-next
-  fix t
-  assume "t \<in> trans m" and "src t \<in> S"
-  with step show "dst t \<in> S" unfolding successors_def by auto
-qed
+  using s base step by (induct s) (auto simp: successors_def)
 
-text {* Next we enunciate and prove a similar lemma for predicates. In a LTS @{text "m"}, 
-if every initial state
-statisfies some predicate @{text "P"} and, for each transition, whenever the source state
-satisfies @{text "P"}, the destination state also satisfies @{text "P"}, then all the
-reachable states satisfy @{text "P"} (and this is an invariant of the LTS). *}
-lemma reachable_induct_predicate:
-  assumes s: "s \<in> states m"
-      and base: "\<forall>s \<in> init m. P s"
-      and step: "\<forall>t \<in> trans m. P (src t) \<longrightarrow> P (dst t)"
-  shows "P s"
-proof -
-  from s have "s \<in> { s . P s}" (is "s \<in> ?S")
-  proof (rule reachable_induct_set)
-    from base show "init m \<subseteq> ?S" by auto
-  next
-    from step show "successors m ?S \<subseteq> ?S" by (auto simp: successors_def)
-  qed
-  thus ?thesis ..
-qed
+text {*
+  The following lemma is similar but stated in terms of a predicate.
+  It contains the principle for proving invariants.
+*}
+lemmas reachable_induct_predicate = states.induct
+
 
 subsection {* Behavior *}
 
-subsubsection {* Internal behavior *}
+text {* 
+  Two views of (finitary) behavior are formalized. The first view is
+  the internal behavior: a \emph{run} is a sequence of transitions such
+  that for any two consecutive transitions, the source state of the
+  second one is the destination state of the first one.
 
-text {* Two views of behavior are formalized. The first view is the internal behavior, and
-corresponds to the set of possible executions. An execution is a sequence of transitions, such
-that two consecutive transitions have coincident state. We introduce the abbreviation @{text "Run"}
-to name the type for executions: *}
+  The second, external view of behavior, projects transitions to their
+  labels: only the name of the event is recorded whereas states are
+  abstracted from.
+*}
+
+subsubsection {* Internal behaviour *}
 
 type_synonym ('st, 'ev) Run = "('st, 'ev) Tr list"
 
-text {* The inductive set @{text "runs"}
-denotes all possible executions of a given LTS @{text "L"}. There are two base cases, 
-corresponding to the empty execution and to executions with a single transition: *}
+text {* 
+  The inductive set @{text "runs l"} denotes the set of finite executions
+  of the LTS @{text "l"}, viewed as lists of transitions. There are two base 
+  cases, corresponding to the empty execution and to executions with a 
+  single transition whose source state is an initial state.
+*}
 
 inductive_set runs :: "('st, 'ev) LTS \<Rightarrow> ('st, 'ev) Run set"  
-          for m :: "('st, 'ev) LTS" where
-  base: "[] \<in> runs m"
-| start: "\<lbrakk> t \<in> trans m; src t \<in> init m \<rbrakk> \<Longrightarrow> [t] \<in> runs m"
-| step: "\<lbrakk> t \<in> trans m; ts \<in> runs m; ts \<noteq> []; src t = dst (last ts) \<rbrakk> \<Longrightarrow> ts @ [t] \<in> runs m"
+  for l :: "('st, 'ev) LTS" where
+  base: "[] \<in> runs l"
+| start: "\<lbrakk> t \<in> trans l; src t \<in> init l \<rbrakk> \<Longrightarrow> [t] \<in> runs l"
+| step: "\<lbrakk> t \<in> trans l; ts \<in> runs l; ts \<noteq> []; src t = dst (last ts) \<rbrakk> \<Longrightarrow> ts @ [t] \<in> runs l"
 
-inductive_cases empty_run : "[] \<in> runs m"
-inductive_cases one_step_run : "[t] \<in> runs m"
-inductive_cases multi_step_run : "ts @ [t] \<in> runs m"
+inductive_cases empty_run : "[] \<in> runs l"
+inductive_cases one_step_run : "[t] \<in> runs l"
+inductive_cases multi_step_run : "ts @ [t] \<in> runs l"
 
-text {* The following lemma states that for any run $ts$ of a LTS $m$, such that $ts$ is not the 
-empty run, then the source state of the first transition is an initial state of $m$. *}
+text {* 
+  The following lemma states that for any non-empty run @{text ts} of an LTS @{text l},
+  the source state of the first transition is an initial state of @{text l}.
+*}
 
-lemma "ts \<in> runs m \<Longrightarrow> ts \<noteq> [] \<Longrightarrow> src (hd ts) \<in> init m"
-by (induct rule: runs.induct) auto
+lemma "ts \<in> runs l \<Longrightarrow> ts \<noteq> [] \<Longrightarrow> src (hd ts) \<in> init l"
+  by (induct rule: runs.induct, auto)
 
-subsubsection {* External behavior *}
 
-text {* The external, or observable, behavior of a LTS is restricted to the events labeling its 
-transitions. We give the name @{text "Trace"} to the type of event lists: *}
+subsubsection {* External behavior. *}
+
+text {* 
+  The external, or observable, behavior of a LTS is obtained by
+  projecting the internal behavior to the events labeling its 
+  transitions. We call this a \emph{trace} of the LTS.
+*}
 
 type_synonym 'ev Trace = "'ev list"
 
-text {* We define the \emph{trace} of a run to be the sequence of events along that run: *}
-
-definition trace_of_run :: "('st, 'ev) Run \<Rightarrow> 'ev Trace" where
-  "trace_of_run ts = map lbl ts"
-
-text {* We then define the \emph{traces} of an LTS from the corresponding runs: *}
-
 definition traces :: "('st, 'ev) LTS \<Rightarrow> 'ev Trace set" where
-  "traces m \<equiv> trace_of_run ` (runs m)"
+  "traces l \<equiv> (map lbl) ` (runs l)"
 
 end
 
