TraceRefinement.thy
@@ -1,6 +1,6 @@
 theory TraceRefinement
 
-imports Main Simulation
+imports Simulation
 
 begin
 
@@ -17,10 +17,10 @@ lemma lts_refines_trans: "\<lbrakk>l \<sqsupseteq> l'; l' \<sqsupseteq> l''\<rbr
 
 lemma 
   assumes "l \<preceq> l'" "ts \<in> runs l"
-  obtains r ts' where "ts' \<in> runs l'" "sim_run r ts ts'"
+  obtains r ts' where "ts' \<in> runs l'" "(ts, ts') \<in> sim_run r"
   using assms unfolding simulates_def by (metis sim_run)
 
-theorem "l' \<preceq> l \<Longrightarrow> l \<sqsubseteq> l'" 
+theorem "l \<preceq> l' \<Longrightarrow> l' \<sqsubseteq> l" 
   unfolding simulates_def refines_def by (metis sim_trace_inclusion)
 
 end
